interface for LowParse.Bytes

src/lowparse/LowParse.Bytes.fsti
@@ -3,27 +3,25 @@ module LowParse.Bytes
 module Seq = FStar.Seq
 module U8 = FStar.UInt8
 
-let bytes_equal (b1 b2: bytes) : GTot Type0 =
-  Seq.length b1 == Seq.length b2 /\
-  (forall (i: nat { i < Seq.length b1 } ) . {:pattern (Seq.index b1 i); (Seq.index b2 i) } U8.v (Seq.index b1 i) == U8.v (Seq.index b2 i))
+type byte = U8.byte
+type bytes = Seq.seq byte
 
-let bytes_equal_intro (b1 b2: bytes) : Lemma
+val bytes_equal (b1 b2: bytes) : GTot Type0
+
+val bytes_equal_intro (b1 b2: bytes) : Lemma
   (requires (
     Seq.length b1 == Seq.length b2 /\
   (forall (i: nat { i < Seq.length b1 } ) . U8.v (Seq.index b1 i) == U8.v (Seq.index b2 i))
   ))
   (ensures (bytes_equal b1 b2))
   [SMTPat (bytes_equal b1 b2)]
-= ()
 
-let bytes_equal_refl (b1 b2: bytes) : Lemma
+val bytes_equal_refl (b1 b2: bytes) : Lemma
   (requires (b1 == b2))
   (ensures (b1 `bytes_equal` b2))
   [SMTPat (bytes_equal b1 b2)]
-= ()
 
-let bytes_equal_elim (b1 b2: bytes) : Lemma
+val bytes_equal_elim (b1 b2: bytes) : Lemma
   (requires (b1 `bytes_equal` b2))
   (ensures (b1 == b2))
   [SMTPat (b1 `bytes_equal` b2)]
-= assert (b1 `Seq.equal` b2)
